removed the `part` function and its lemmas

heap.lean
@@ -86,27 +86,6 @@ else heap.delete (p+1) n h q
 
 infix ` <+ `:54 := left_combine
 
-section noncomp
-
-local attribute [instance] classical.prop_decidable
-
-noncomputable def part (h₀ h₁ : heap) : option heap :=
-if Hd : h₀ ## h₁
-then some (part' h₀ h₁)
-else none
-
-end noncomp
-
-@[simp]
-lemma heap_emp_part (h : heap)
-: part heap.emp h = some h :=
-by simp [part]
-
-@[simp]
-lemma part_heap_emp (h : heap)
-: part h heap.emp = some h :=
-by simp [part]
-
 @[symm]
 lemma disjoint_symm {h₀ h₁ : heap}
   (h : h₀ ## h₁)
@@ -119,29 +98,6 @@ lemma part_comm' {h₀ h₁ : heap}
 begin
   funext p, unfold part',
   cases h p with h h ; simp [h],
-end
-
-lemma part_comm (h₀ h₁ : heap)
-: part h₀ h₁ = part h₁ h₀ :=
-begin
-  unfold part,
-  cases classical.em (h₀ ## h₁) with H H,
-  { have H' := disjoint_symm H,
-    simp [dif_pos,H,H',part_comm' H] },
-  { have H' := mt disjoint_symm H,
-    simp [dif_neg,H,H'] }
-end
-
-lemma disjoint_of_part {h h₀ h₁ : heap}
-  (HH : some h = part h₀ h₁)
-: h₀ ## h₁ :=
-begin
-  unfold part at HH,
-  apply classical.by_contradiction _,
-  intro H,
-  rw [dif_neg] at HH,
-  { contradiction },
-  { assumption }
 end
 
 lemma part_disjoint_assoc_left {h₀ h₁ h₂ : heap}
@@ -176,17 +132,6 @@ lemma eq_emp_of_part' (hp a : heap)
 : a = part' a hp ↔ hp = heap.emp :=
 sorry
 
-@[simp]
-lemma eq_emp_of_part (hp a : heap)
-: some a = part a hp ↔ hp = heap.emp :=
-sorry
-
-@[simp]
-lemma part'_eq_emp (a b : heap)
-  (h  : a ## b)
-: part' a b = heap.emp ↔ a = heap.emp ∧ b = heap.emp :=
-sorry
-
 lemma part'_part'_assoc {h₀ h₁ h₂ : heap}
   (Hdisj₀ : h₀ ## h₁)
   (Hdisj₁ : h₁ ## h₂)
@@ -194,77 +139,6 @@ lemma part'_part'_assoc {h₀ h₁ h₂ : heap}
   (Hdisj₃ : h₀ ## part' h₁ h₂)
 : part' (part' h₀ h₁) h₂ Hdisj₂ = part' h₀ (part' h₁ h₂) Hdisj₃ :=
 sorry
-
-lemma part'_part_assoc {h₀ h₁ h₂ : heap}
-  (Hdisj : h₀ ## h₁)
-  (Hdisj' : h₁ ## h₂)
-: part (part' h₀ h₁) h₂ = part h₀ (part' h₁ h₂) :=
-begin
-  unfold part,
-  cases classical.em (part' h₀ h₁ Hdisj ## h₂) with h h,
-  { have h' : (h₀ ## part' h₁ h₂ Hdisj') := part_disjoint_assoc_left _ _ h,
-    simp [dif_pos,h,h'],
-    apply congr_arg,
-    funext p, simp [part',or_else_assoc], },
-  { have h' : ¬ (h₀ ## part' h₁ h₂ Hdisj'),
-    { rw part_comm',
-      apply mt disjoint_symm,
-      apply mt (part_disjoint_assoc_left _ _),
-      apply mt disjoint_symm,
-      rw part_comm',
-      apply h,
-      apply disjoint_symm Hdisj },
-    simp [dif_neg,h,h'] }
-end
-
-lemma part'_of_part {h h₀ h₁ : heap}
-  (H : some h = part h₀ h₁)
-: h = part' h₀ h₁ (disjoint_of_part H) :=
-begin
-  unfold part at H, dedup,
-  simp [dif_pos,disjoint_of_part H] at H_1,
-  injection H_1,
-end
-
-def heap.le (hp₀ hp₁ : heap) : Prop :=
-∃ hp, some hp₁ = part hp₀ hp
-
-instance : has_le heap :=
-⟨ heap.le ⟩
-
-instance : partial_order heap :=
-{ le := heap.le
-, le_refl := by { intro x, existsi heap.emp, simp [part_comm] }
-, le_trans := by { introv,
-                   simp [has_le.le,heap.le],
-                   intros hp₀ h₀ hp₁ h₁,
-                   have : hp₀ ## hp₁, admit,
-                   existsi part' hp₀ hp₁,
-                   rw [h₁,part'_of_part h₀,part'_part_assoc], }
-, le_antisymm := by { introv,
-                      simp [has_le.le,heap.le],
-                      intros hp₀ h₀ hp₁ h₁,
-                      have h : hp₀ ## hp₁, admit,
-                      rw [part'_of_part h₀,part'_part_assoc _ h
-                         ,eq_emp_of_part,part'_eq_emp] at h₁,
-                      simp [h₁.left] at h₀,
-                      injection h₀, subst b, }
-}
-
-lemma part'_delete_maplet (p : pointer) (v : word) (hp : heap)
-  (h : heap.delete p 1 hp ## maplet p v)
-  (h' : maplet p v ≤ hp)
-: part' (heap.delete p 1 hp) (maplet p v) = hp :=
-begin
-  funext p',
-  by_cases (p = p') with h,
-  { simp [part', heap.delete, maplet, if_pos, h],
-    unfold has_le.le heap.le at h',
-    cases h' with hp' h',
-    rw [part'_of_part h',part',maplet,if_pos h],
-    simp },
-  { simp [part', heap.delete, maplet, if_neg, h] }
-end
 
 lemma delete_part'_heap_mk {p : pointer} {vs : list word} {hp : heap}
   (h : heap.mk p vs ## hp)
@@ -294,62 +168,6 @@ begin
   rw part_comm', apply H₀,
 end
 
-noncomputable def parts : list heap → option heap
- | [] := some heap.emp
- | (x :: xs) :=
-do ys ← parts xs,
-   part x ys
-
-lemma parts_congr {hp₀ hp₁ : list heap}
-  (H : hp₀ ~ hp₁)
-: parts hp₀ = parts hp₁ :=
-begin
-  induction H,
-  case perm.nil
-  { refl },
-  case perm.skip
-  { unfold parts,
-    rw ih_1, },
-  case perm.swap
-  { unfold parts,
-    simp [monad.bind_assoc],
-    apply congr_arg,
-    funext z,
-    unfold part,
-    cases classical.em (disjoint x z) with h h
-    ; cases classical.em (disjoint y z) with h' h'
-    ; simp [h,h']
-    ; simp [bind,option.bind],
-    { rw [part_comm',← part'_part_assoc h',part_comm], },
-    { unfold part,
-      rw dif_neg, intros h'', apply h',
-      apply disjoint_disjoint_left,
-      symmetry, assumption },
-    { unfold part,
-      rw dif_neg, intros h'', apply h,
-      apply disjoint_disjoint_left,
-      symmetry, assumption },  },
-  case perm.trans
-  { cc }
-end
-
-lemma part'_eq_parts_app_of_parts_parts {hp₀ hp₁ : heap} {hs₀ hs₁ : list heap}
-  (H₀ : hp₀ ## hp₁)
-  (H₁ : some hp₀ = parts hs₀)
-  (H₂ : some hp₁ = parts hs₁)
-: some (part' hp₀ hp₁) = parts (hs₀ ++ hs₁) :=
-sorry
-
-lemma part_eq_parts_app_of_parts_parts {hp₀ hp₁ : heap} {hs₀ hs₁ : list heap}
-  (H₁ : some hp₀ = parts hs₀)
-  (H₂ : some hp₁ = parts hs₁)
-: part hp₀ hp₁ = parts (hs₀ ++ hs₁) :=
-sorry
-
-lemma parts_singleton (hp : heap)
-: some hp = parts [hp] :=
-sorry
-
 def heap.insert (hp : heap) (p : pointer) (v : word) : heap
  | q := if p = q then some v else hp q
 
@@ -362,75 +180,3 @@ sorry
 lemma maplet_insert_disjoint_iff (p : pointer) (v v' : word) (hp : heap)
 : (maplet p v).insert p v' ## hp ↔ maplet p v ## hp :=
 sorry
-
-namespace tactic.interactive
-
-open tactic
-
-/-- Given `h : heap`, find `hs : list heap` such that `some h = parts hs` -/
-meta def flat_heap_expr : expr → tactic (dlist expr × expr)
- | `(part' %%h₀ %%h₁ %%Hd) :=
-do (hs₀,p₀) ← flat_heap_expr h₀,
-   (hs₁,p₁) ← flat_heap_expr h₁,
-   p ← to_expr ``(part'_eq_parts_app_of_parts_parts %%Hd %%p₀ %%p₁),
-   return (hs₀ ++ hs₁,p)
- | h :=
-do p ← to_expr ``(parts_singleton %%h),
-   return (dlist.singleton h, p )
-
-/-- Given `h : option heap`, find `hs : list heap` such that `h = parts hs` -/
-meta def flat_opt_heap_expr : expr → tactic (dlist expr × expr)
- | `(part %%h₀ %%h₁) :=
-do (hs₀,p₀) ← flat_heap_expr h₀,
-   (hs₁,p₁) ← flat_heap_expr h₁,
-   p ← to_expr ``(part_eq_parts_app_of_parts_parts %%p₀ %%p₁),
-   return (hs₀ ++ hs₁,p)
- | e := fail "expecting expression of the form `part ?m ?m`"
-
-meta def flatten_heap : tactic unit :=
-do t ← target,
-   (e₀,e₁) ← expr.is_eq t,
-   (ls,p) ← flat_heap_expr e₁,
-   h ← note `h none p,
-   `[simp at h],
-   asrt ← to_expr ``(some %%e₀ = some %%e₁),
-   h' ← assert `h asrt,
-   tactic.swap,
-   tactic.injection h' >> assumption,
-   h ← get_local `h,
-   rewrite_target h,
-   tactic.clear h,
-   return ()
-
-meta def eq_heap : tactic unit := do
-do t ← target,
-   (e₀, e₁) ← expr.is_eq t,
-   (_,p₀) ← flat_opt_heap_expr e₀,
-   (_,p₁) ← flat_opt_heap_expr e₁,
-   rewrite_target p₀,
-   rewrite_target p₁,
-   `[apply parts_congr, simp],
-   prove_perm
-
-section
-
-variables {hp hp₀ hp₁ hp₂ hp₃ : heap}
-variables (d₀₁ : hp₀ ## hp₁)
-variables (d₁₀ : hp₁ ## hp₀)
-variables (d₂₃ : hp₂ ## hp₃)
-variables (d₀₁₂₃ : disjoint (part' hp₀ hp₁ d₀₁) (part' hp₂ hp₃ d₂₃))
-variables (h : some hp = parts [hp₀,hp₁,hp₂,hp₃])
-include d₀₁ d₁₀ d₂₃ d₀₁₂₃ h
-example : hp = part' (part' hp₀ hp₁) (part' hp₂ hp₃) d₀₁₂₃ :=
-begin
-  flatten_heap,
-  apply h,
-end
-
-example : part  (part' hp₁ hp₀) (part' hp₂ hp₃) = part (part' hp₂ hp₃) (part' hp₀ hp₁)  :=
-begin
-  eq_heap
-end
-end
-
-end tactic.interactive
